src/feather_model/basic.lean
@@ -1,0 +1,159 @@
+import feather_logic.basic
+import order.extension.well
+
+universe u
+
+namespace feather_model
+
+open_locale classical
+
+/-- The type of variables in our model. -/
+def V : Type u := ulift ℕ
+
+/--
+A term in our model.
+
+* `var v` is the term representing the variable `v`.
+* `ty α` is the Lean type `α`.
+* `obj α x` is a Lean object of type `α` and value `x : α`.
+* `apply f x` is the term representing function application of `f` on `x`.
+-/
+inductive mterm : Type (u + 1)
+| var : V.{u} → mterm
+| ty : Type u → mterm
+| obj : Π (α : Type u), α → mterm
+| apply : mterm → mterm → mterm
+
+namespace mterm
+
+def bound : Π (e : mterm), finset V
+| (var v) := {v}
+| (ty α) := ∅
+| (obj α x) := ∅
+| (apply f x) := bound f ∪ bound x
+
+-- A convenient instance to use instead of explicitly calling `bound` all the time.
+instance mterm_has_mem : has_mem V mterm := ⟨λ v e, v ∈ bound e⟩
+
+def subst (v : V) (e : mterm) : Π (f : mterm), mterm
+| (var w) := if v = w then e else var w
+| (ty α) := ty α
+| (obj α x) := obj α x
+| (apply f x) := apply (subst f) (subst x)
+
+def has_type : Π (e f : mterm), Prop
+| (obj α x) (ty β) := α = β
+| _ _ := false
+
+end mterm
+
+open mterm
+
+section interpretation
+
+/-! Given a context, which here means a  `finset (V × mterm)`, we produce the set of all
+*interpretations* of that context: substitutions of Lean objects for these variables
+that satisfy the given context. -/
+
+/--
+We establish a relation on judgments `V × mterm`.
+If `v` occurs bound in a term `f`, then `(v, e)` must precede `(w, f)`.
+
+On a plain context `finset (V × mterm)`, if the transitive closure of this relation forms a
+strict partial order, we can sort the judgments and provide a set of interpretations for it by
+iteratively substituting along this order.
+-/
+def immediately_precedes (a b : V × mterm) : Prop := a.1 ∈ b.2
+
+/-- A list of substitutions to perform to yield a interpretation of a collection of variables. -/
+@[reducible] def interpretation := list (V × mterm)
+
+/-- Given an interpretation, evaluate this term. -/
+def interpretation.interpret (I : interpretation) (e : mterm) : mterm :=
+list.foldl (λ (f : mterm) (i : V × mterm), subst i.1 i.2 f) e I
+
+/-- A collection of assumptions `V × mterm` is *sortable* if they can be ordered in such a way
+where each variable occurs only in substitutions later in the order. -/
+def interpretation.sortable (C : finset (V × mterm)) : Prop :=
+well_founded (λ a b : C, immediately_precedes a.val b.val)
+
+/-- Assuming a context is sortable, produce a linear order for it. -/
+noncomputable def interpretation.sort_order (C : finset (V × mterm))
+  (h : interpretation.sortable C) : linear_order C :=
+well_founded.well_order_extension h
+
+/-- Assuming that a context is sortable, sort it. The precise sort chosen is arbitrary. -/
+noncomputable def interpretation.sort (C : finset (V × mterm)) (h : interpretation.sortable C) :
+  list (V × mterm) :=
+(finset.sort (interpretation.sort_order C h).le C.attach).map subtype.val
+
+/-- Substitutes the term `e` for the variable `v`. If the context contains an assumption `v : α`,
+it is removed. -/
+def interpretation.subst (v : V) (e : mterm) (I : list (V × mterm)) : list (V × mterm) :=
+(I.filter (λ x : V × mterm, x.1 = v)).map (prod.map id (subst v e))
+
+lemma interpretation.subst_length (v : V) (e : mterm) (I : interpretation) :
+  (interpretation.subst v e I).length ≤ I.length :=
+begin
+  unfold interpretation.subst,
+  rw list.length_map,
+  exact list.length_filter_le _ _,
+end
+
+/-- The set of interpretations of a typing judgment `e : type`. -/
+def interpretations (v : V) : Π (type : mterm), set interpretation
+| (ty α) := ⋃ (x : α), {[⟨v, mterm.obj α x⟩]}
+| _ := ∅
+
+def interpretations' : Π (C : list (V × mterm)), set interpretation
+| [] := {[]}
+| (x :: xs) := ⋃ (I ∈ interpretations x.1 x.2),
+    have (interpretation.subst x.1 x.2 xs).length < (x :: xs).length,
+    from lt_of_le_of_lt (interpretation.subst_length x.1 x.2 xs) (lt_add_one _),
+    (λ J, I ++ J) '' interpretations' (interpretation.subst x.1 x.2 xs)
+using_well_founded { rel_tac := λ _ _, `[exact ⟨_, measure_wf list.length⟩] }
+
+def plain_context.interpretations (C : plain_context mterm V) : set interpretation :=
+if h : interpretation.sortable C.Γ then interpretations' (interpretation.sort _ h) else ∅
+
+def rir_context.interpretations (C : rir_context mterm V) : set interpretation :=
+if h : interpretation.sortable (C.Γ ∪ C.Ξ)
+then interpretations' (interpretation.sort _ h) else ∅
+
+def runtime_context.interpretations (C : runtime_context mterm V) : set interpretation :=
+if h : interpretation.sortable (C.Γ ∪ C.Θ.to_finset ∪ C.Ξ)
+then interpretations' (interpretation.sort _ h) else ∅
+
+end interpretation
+
+def runtime_judgments (J : runtime_judgment mterm V) : Prop :=
+∀ (I : interpretation), I ∈ J.ctx.interpretations → (I.interpret J.e).has_type (I.interpret J.type)
+
+def rir_judgments (J : rir_judgment mterm V) : Prop :=
+∀ (I : interpretation), I ∈ J.ctx.interpretations → (I.interpret J.e).has_type (I.interpret J.type)
+
+def defeq (C : plain_context mterm V) (x y α : mterm) : Prop :=
+∀ (I : interpretation), I ∈ C.interpretations →
+  I.interpret x = I.interpret y ∧ (I.interpret x).has_type (I.interpret α)
+
+def sort : sort_name → mterm.{u}
+| (sort_name.type n) := ty pempty
+| sort_name.prop := ty (ulift Prop)
+| sort_name.region := ty punit
+
+def representable (C : finset (V × mterm)) (e : mterm) : mterm.{u} :=
+mterm.obj (ulift Prop) ⟨false⟩
+
+instance : term_struct mterm := {
+  V := V,
+  var := var,
+  bound := bound,
+  subst := subst,
+  runtime_judgments := runtime_judgments,
+  rir_judgments := rir_judgments,
+  defeq := defeq,
+  sort := sort,
+  representable := representable,
+}
+
+end feather_model
